Coq. Working on construction of certification graph.

Coq/src/SimRel.v
@@ -1,4 +1,4 @@
-Require Import Program.Basics.
+Require Import Program.Basics Omega.
 Require Import Coq.Logic.FunctionalExtensionality Classical_Prop.
 From hahn Require Import Hahn.
 From promising Require Import Basic.
@@ -31,6 +31,7 @@ Section SimRel.
   Notation "'Grf'" := (G.(rf)).
   Notation "'Gvf'" := (G.(Gvf)).
   Notation "'Gco'" := (G.(co)).
+  Notation "'Grmw'" := (G.(rmw)).
   Notation "'Stid'" := (S.(ES.tid)).
   Notation "'Slab'" := (S.(ES.lab)).
   Notation "'Sloc'" := (loc S.(ES.lab)).
@@ -40,6 +41,7 @@ Section SimRel.
   Notation "'Scf'" := (S.(ES.cf)).
   Notation "'Sew'" := (S.(ES.ew)).
   Notation "'Sjf'" := (S.(ES.jf)).
+  Notation "'Srmw'" := (S.(ES.rmw)).
   Notation "'Svf'" := (Svf S Weakestmo).
   Notation "'Gtid_' t" := (fun x => tid x = t) (at level 1).
   Notation "'Stid_' t" := (fun x => Stid x = t) (at level 1).
@@ -48,7 +50,7 @@ Section SimRel.
   Notation "'SR'" := (fun a => is_true (is_r Slab a)).
 
   Definition pc thread :=
-    f □₁ C ∩₁ Stid_ thread \₁ dom_rel (Ssb ⨾ ⦗ f □₁ C ⦘).
+    C ∩₁ Gtid_ thread \₁ dom_rel (Gsb ⨾ ⦗ C ⦘).
 
   Definition thread_lts (tid : thread_id) : Language.t :=
     @Language.mk
@@ -62,18 +64,16 @@ Section SimRel.
                         (INK : K (cont, existT _ lang state)),
         lang = thread_lts (ES.cont_thread S cont);
 
-      continit : forall thread (state : (thread_lts thread).(Language.state))
-                        (INK : K (ES.CInit thread, existT _ _ state)),
-          exists lprog,
-            ⟪ INPROG : IdentMap.find thread prog = Some lprog ⟫ /\
+      continit : forall thread lprog
+                        (INPROG : IdentMap.find thread prog = Some lprog),
+          exists (state : (thread_lts thread).(Language.state)),
+            ⟪ INK : K (ES.CInit thread, existT _ _ state) ⟫ /\
             ⟪ INITST : state = (thread_lts thread).(Language.init) lprog ⟫;
 
-      contpc : forall e (state : (thread_lts (Stid e)).(Language.state))
-                      (PC : pc (Stid e) e)
-                      (INK : K (ES.CEvent e, existT _ _ state)),
-                @sim_state G sim_normal C (Stid e) state;
-      
-      (* TODO: for a certification graph will need smth close to `contpc`. *)
+      contpc : forall e (state : (thread_lts (Gtid e)).(Language.state))
+                      (PC : pc (Gtid e) e)
+                      (INK : K (ES.CEvent (f e), existT _ _ state)),
+                @sim_state G sim_normal C (Gtid e) state;
     }.
   
   Definition event_to_act (e : eventid) : actid :=
@@ -97,15 +97,17 @@ Section SimRel.
                        (EE : GE (ThreadEvent thread n)),
           GE (ThreadEvent thread m);
       tccoh : tc_coherent G sc TC;
+      rmwclos : forall r w (RMW : Grmw r w), C r <-> C w;
       swf   : ES.Wf S;
       scons : @es_consistent S Weakestmo;
       
       scont : simrel_cont;
 
       fgtrip : ⦗ fdom ⦘ ⨾ ↑ (compose g f) ⊆ eq;
-      gew : g □ Sew ⊆ eq;
-      gco : g □ Sco ⊆ Gco;
-      gjf : g □ Sjf ⊆ Gvf;
+      gew  : g □ Sew  ⊆ eq;
+      gco  : g □ Sco  ⊆ Gco;
+      gjf  : g □ Sjf  ⊆ Gvf;
+      grmw : g □ Srmw ⊆ Grmw;
 
       fco : f □ ⦗ fdom ⦘ ⨾ Gco ⨾ ⦗ fdom ⦘ ⊆ Sco;
 
@@ -235,5 +237,55 @@ Section SimRel.
     Proof.
       (* TODO. It should follow from glab and definition of g. *)
     Admitted.
+    
+    Lemma cont_tid_state e (EE : GE e) (NINIT : ~ is_init e) :
+      exists (state : (thread_lts (tid e)).(Language.state)) c,
+        << QQ : K (c, existT _ _ state) >> /\
+        << SSTATE : @sim_state G sim_normal C (tid e) state >>.
+    Proof.
+      set (HH := EE).
+      apply GPROG in HH. desf.
+      destruct (IdentMap.find (Gtid e) prog) as [lprog|] eqn:AA.
+      2: { apply IdentMap.Facts.in_find_iff in HH. desf. }
+      generalize AA. generalize (Gtid e).
+      clear e EE NINIT HH AA.
+      intros thread AA.
+      destruct (classic (exists e, pc thread e)) as [[e PC]|NPC].
+      2: { edestruct (continit (scont SRC)) as [state]; eauto.
+           desf.
+           eexists. eexists.
+           splits; eauto.
+           red. splits; ins.
+           2: { symmetry in AA.
+                eapply GPROG in AA. desf.
+                cdes AA. exists s.
+                red. splits; auto.
+                  by rewrite PEQ. }
+           split; intros XX; [|omega].
+           exfalso. apply NPC.
+           admit. }
+      assert (thread = Gtid e); subst.
+      { red in PC. generalize PC. basic_solver. }
+      assert (C e) as CE by apply PC.
+      assert (~ dom_rel Grmw e) as NRMW.
+      { intros [w RMW].
+        eapply PC. exists w.
+        apply seq_eqv_r. split.
+        { apply rmw_in_sb; auto. apply SRC. }
+          by apply rmwclos with (r:=e) (w:=w). }
+      assert (~ dom_rel Srmw (f e)) as NSRMW.
+      { intros [w RMW].
+        apply NRMW. exists (g w).
+        apply SRC.(grmw).
+        arewrite (e = g (f e)).
+        { apply SRC.(fgtrip). apply seq_eqv_l.
+            by split; [left|]. }
+        (* TODO: simplify *)
+        eexists. eexists. splits; eauto. }
+      admit.
+      (* eapply contpc in PC. *)
+      (* 2: by apply SRC. *)
+   Admitted.
+
   End Properties.
 End SimRel.
